while checker in the new interface

pulse/lib/steel/pulse/Pulse.Checker.While.fst
@@ -7,6 +7,7 @@ open Pulse.Syntax
 open Pulse.Typing
 open Pulse.Checker.Pure
 open Pulse.Checker.Common
+open Pulse.Prover
 
 module P = Pulse.Syntax.Printer
 module FV = Pulse.Typing.FV
@@ -14,35 +15,96 @@ module Framing = Pulse.Checker.Framing
 module Metatheory = Pulse.Typing.Metatheory
 module RU = Pulse.RuntimeUtils
 
-// let while_cond_comp_typing (#g:env) (u:universe) (x:ppname) (ty:term) (inv_body:term)
-//                            (inv_typing:tot_typing g (tm_exists_sl u (as_binder ty) inv_body) tm_vprop)
-//   : Metatheory.comp_typing_u g (comp_while_cond x inv_body)
-//   = Metatheory.admit_comp_typing g (comp_while_cond x inv_body)
+let while_cond_comp_typing (#g:env) (u:universe) (x:ppname) (ty:term) (inv_body:term)
+                           (inv_typing:tot_typing g (tm_exists_sl u (as_binder ty) inv_body) tm_vprop)
+  : Metatheory.comp_typing_u g (comp_while_cond x inv_body)
+  = Metatheory.admit_comp_typing g (comp_while_cond x inv_body)
 
-// let while_body_comp_typing (#g:env) (u:universe) (x:ppname) (ty:term) (inv_body:term)
-//                            (inv_typing:tot_typing g (tm_exists_sl u (as_binder ty) inv_body) tm_vprop)
-//   : Metatheory.comp_typing_u g (comp_while_body x inv_body)
-//   = Metatheory.admit_comp_typing g (comp_while_body x inv_body)
+let while_body_comp_typing (#g:env) (u:universe) (x:ppname) (ty:term) (inv_body:term)
+                           (inv_typing:tot_typing g (tm_exists_sl u (as_binder ty) inv_body) tm_vprop)
+  : Metatheory.comp_typing_u g (comp_while_body x inv_body)
+  = Metatheory.admit_comp_typing g (comp_while_body x inv_body)
 
-// #push-options "--fuel 0 --ifuel 2 --z3rlimit_factor 10 --split_queries no --query_stats"
-// let check_while
-//   (allow_inst:bool)
-//   (g:env)
-//   (t:st_term{Tm_While? t.term})
-//   (pre:term)
-//   (pre_typing:tot_typing g pre tm_vprop)
-//   (post_hint:post_hint_opt g)
-//   (frame_pre:bool)
-//   (check':bool -> check_t)
-//   : T.Tac (checker_result_t g pre post_hint frame_pre) =
-//   if not frame_pre
-//   then T.fail "check_while, frame_pre is false, bailing";
-//   let g = push_context "while loop" t.range g in
-//   let Tm_While { invariant=inv; condition=cond; body; condition_var } = t.term in
-//   let (| ex_inv, inv_typing |) =
-//     check_vprop (push_context "invariant" (term_range inv) g) 
-//                 (tm_exists_sl u0 { binder_ppname=condition_var; binder_ty=tm_bool } inv)
-//   in
+#push-options "--fuel 0 --ifuel 1 --z3rlimit_factor 4"
+let check_while
+  (g:env)
+  (t:st_term{Tm_While? t.term})
+  (pre:term)
+  (pre_typing:tot_typing g pre tm_vprop)
+  (post_hint:post_hint_opt g)
+  (check:check_t)
+  : T.Tac (checker_result_t g pre post_hint) =
+
+  let g = push_context "while loop" t.range g in
+  let Tm_While { invariant=inv; condition=cond; body; condition_var } = t.term in
+  let (| ex_inv, inv_typing |) =
+    check_vprop (push_context "invariant" (term_range inv) g) 
+                (tm_exists_sl u0 { binder_ppname=condition_var; binder_ty=tm_bool } inv)
+  in
+
+  if not (Tm_ExistsSL? ex_inv.t)
+  then fail g None "Typechecked invariant is not an exists";
+
+  let Tm_ExistsSL u {binder_ppname=nm; binder_ty=ty} inv = ex_inv.t in
+
+  if not (eq_tm ty tm_bool) ||
+     not (eq_univ u u0)
+  then fail g (Some nm.range) "While loop invariant exists but its witness type is not bool";
+
+  let while_cond_comp_typing = while_cond_comp_typing u nm ty inv inv_typing in
+  let (| res_typing, cond_pre_typing, x, post_typing |) =
+    Metatheory.(st_comp_typing_inversion (comp_typing_inversion while_cond_comp_typing))
+  in
+  let while_cond_hint : post_hint_for_env g =
+    post_hint_from_comp_typing while_cond_comp_typing
+  in
+
+  let (| cond, cond_comp, cond_typing |) =
+    let r = check
+      (push_context "while condition" cond.range g)
+      (comp_pre (comp_while_cond nm inv))
+      cond_pre_typing
+      (Some while_cond_hint)
+      cond in
+    apply_checker_result_k r
+  in
+  if eq_comp cond_comp (comp_while_cond nm inv)
+  then begin
+    let while_body_comp_typing = while_body_comp_typing u nm ty inv inv_typing in
+    let (| res_typing, body_pre_typing, x, post_typing |) = 
+      Metatheory.(st_comp_typing_inversion (comp_typing_inversion while_body_comp_typing))
+    in
+    let while_post_hint : post_hint_for_env g =
+      post_hint_from_comp_typing while_body_comp_typing
+    in
+    let (| body, body_comp, body_typing |) =
+      let r = check
+        (push_context "while body" body.range g)
+        (comp_pre (comp_while_body nm inv))
+        body_pre_typing
+        (Some while_post_hint)
+        body in
+      apply_checker_result_k r in
+    if eq_comp body_comp (comp_while_body nm inv)
+    then
+      let d = T_While g inv cond body inv_typing cond_typing body_typing in
+      repack (try_frame_pre pre_typing d) post_hint t.range
+    else fail g None
+          (Printf.sprintf "Could not prove the inferred type of the while body matches the annotation\n\
+                           Inferred type = %s\n\
+                           Annotated type = %s\n"
+                           (P.comp_to_string body_comp)
+                           (P.comp_to_string (comp_while_body nm inv)))
+  end
+  else fail g None 
+         (Printf.sprintf "Could not prove that the inferred type of the while condition matches the annotation\n\
+                          Inferred type = %s\n\
+                          Annotated type = %s\n"
+                          (P.comp_to_string cond_comp)
+                          (P.comp_to_string (comp_while_cond nm inv)))
+
+
+
 //   if RU.debug_at_level (fstar_env g) "inference"
 //   then (
 //     T.print (Printf.sprintf "Checking precondition of while loop: %s\n" (P.term_to_string ex_inv))
@@ -50,48 +112,8 @@ module RU = Pulse.RuntimeUtils
 //   match Framing.check_frameable pre_typing ex_inv with
 //   | Inr f -> T.raise (Framing_failure f)
 //   | Inl framing_token ->
-//     match ex_inv.t with
-//     | Tm_ExistsSL u {binder_ppname=nm; binder_ty=ty} inv ->
-//       if not (eq_tm ty tm_bool) ||
-//          not (eq_univ u u0)
-//       then fail g (Some nm.range) "While loop invariant exists but its witness type is not bool"
-//       else begin
-//         let while_cond_comp_typing = while_cond_comp_typing u nm ty inv inv_typing in
-//         let (| res_typing, cond_pre_typing, x, post_typing |) =
-//             Metatheory.(st_comp_typing_inversion (comp_typing_inversion while_cond_comp_typing))
-//         in
-//         let while_cond_hint
-//           : post_hint_for_env g
-//           = post_hint_from_comp_typing while_cond_comp_typing
-//         in
-//         let (| cond, cond_comp, cond_typing |) =
-//           check' allow_inst
-//                  (push_context "while condition" cond.range g)
-//                  cond
-//                  (comp_pre (comp_while_cond nm inv))
-//                  cond_pre_typing
-//                  (Some while_cond_hint)
-//                  frame_pre
-//         in
 //         if eq_comp cond_comp (comp_while_cond nm inv)
 //         then begin
-//           let while_body_comp_typing = while_body_comp_typing u nm ty inv inv_typing in
-//           let (| res_typing, body_pre_typing, x, post_typing |) = 
-//               Metatheory.(st_comp_typing_inversion (comp_typing_inversion while_body_comp_typing))
-//           in
-//           let while_post_hint
-//             : post_hint_for_env g
-//             = post_hint_from_comp_typing while_body_comp_typing
-//           in
-//           let (| body, body_comp, body_typing |) =
-//               check' allow_inst
-//                      (push_context "while body" body.range g)
-//                      body
-//                      (comp_pre (comp_while_body nm inv))
-//                      body_pre_typing
-//                      (Some while_post_hint)
-//                      frame_pre
-//           in
 //           if eq_comp body_comp (comp_while_body nm inv)
 //           then let d = T_While g inv cond body inv_typing cond_typing body_typing in
 //                let (| c, st_d |) = Framing.apply_frame pre_typing d framing_token in
